## This is the research model for the research project Early Modern Professorial Career Patterns - Methodological research on online databases of academic history.

@prefix : <http://pcp-on-web.de/ontology#> .
@prefix pcp: <http://pcp-on-web.de/ontology#> .
@prefix owl: <http://www.w3.org/2002/07/owl#> .
@prefix rdf: <http://www.w3.org/1999/02/22-rdf-syntax-ns#> .
@prefix xml: <http://www.w3.org/XML/1998/namespace> .
@prefix xsd: <http://www.w3.org/2001/XMLSchema#> .
@prefix dc: <http://purl.org/dc/terms/>.
@prefix rdfs: <http://www.w3.org/2000/01/rdf-schema#> .
@base <http://pcp-on-web.de/ontology#> .
@prefix foaf: <http://xmlns.com/foaf/0.1/> .
@prefix gn: <http://www.geonames.org/ontology#> .
@prefix fabio: <http://purl.org/spar/fabio/> .
@prefix gndo: <http://d-nb.info/standards/elementset/gnd#> .
@prefix wgs84: <http://www.w3.org/2003/01/geo/wgs84_pos#> .

<http://pcp-on-web.de/ontology#> rdf:type owl:Ontology ;
	<http://creativecommons.org/ns#attributionName> "AKSW", "HAB", "HTWK" ;
	dc:title "Professorale Karrieremuster der Frühen Neuzeit - Version 0.1 (pcp-on-web)"@de,
  	"Early Modern Professorial Career Patterns - Version 0.1 (pcp-on-web)"@en;
	dc:license "http://creativecommons.org/licenses/by/4.0/" ;
	dc:modified "2021-02-03";
	<http://purl.org/vocab/vann/changes> <https://github.com/pcp-on-web/ontology/commits/master/index.rdf> ;
	<http://purl.org/vocab/vann/preferredNamespacePrefix> "pcp" ;
	<http://purl.org/vocab/vann/preferredNamespaceUri> "http://pcp-on-web.de/ontology#" ;
	<http://usefulinc.com/ns/doap#homepage> <https://pcp-on-web.de/project/> ;
  <http://usefulinc.com/ns/doap#maintainer> <https://pcp-on-web.de/team/JenniferBlanke>, <https://pcp-on-web.de/team/ThomasRiechert> ;
	dc:description "The PCP-on-Web Model defines the research model for the research projekt Early Modern Professorial Career Patterns Methodological research on online databases of academic history.";
	rdfs:label "Professorale Karrieremuster der Frühen Neuzeit - Version 0.1 (pcp-on-web)"@de,
  	"Early Modern Professorial Career Patterns - Version 0.1 (pcp-on-web)"@en;
  	owl:versionInfo "Version 0.1 (inital) - 2021-02-03 - Jennifer Blanke";
  	dc:creator "Jennifer Blanke, Edgard Marx, Thomas Riechert" ;
  	<http://xmlns.com/foaf/0.1/maker> <http://pcp-on-web.de/team/JenniferBlanke> , <http://pcp-on-web.de/team/EdgardMarx> , <http://pcp-on-web.de/team/ThomasRiechert>.

#################################################################
#    Datatypes
#################################################################

###  http://www.w3.org/2001/XMLSchema#date
xsd:date rdf:type rdfs:Datatype .


###  http://www.w3.org/2001/XMLSchema#gDay
xsd:gDay rdf:type rdfs:Datatype .


###  http://www.w3.org/2001/XMLSchema#gMonth
xsd:gMonth rdf:type rdfs:Datatype .


###  http://www.w3.org/2001/XMLSchema#gMonthDay
xsd:gMonthDay rdf:type rdfs:Datatype .


###  http://www.w3.org/2001/XMLSchema#gYear
xsd:gYear rdf:type rdfs:Datatype .


###  http://www.w3.org/2001/XMLSchema#gYearMonth
xsd:gYearMonth rdf:type rdfs:Datatype .		
		
		
#################################################################
#		Classes
#################################################################
	
:AcademicOffice rdf:type owl:Class ;
  rdfs:subClassOf :StageOfLife ;
  rdfs:label "Akademisches Amt"@de, "Academic office"@en ;
	rdfs:comment "Akademische Ämter wie Professor, Rektor, Prorektor, Kanzler, Dekan usw. ."@de, "Academic offices like professor, rector, prorector, chancellor, dean etc.."@en .
		
:Article rdf:type owl:Class ;
  rdfs:subClassOf :Publication ;
  rdfs:subClassOf fabio:Article ;
  rdfs:label "Artikel"@de, "Article"@en ;
	rdfs:comment "Artikel in Periodika wie Journalen, Zeitschriften, Zeitungen oder Magazinen."@de, "Articles published in periodicals like journals, newspapers or magazines."@en .
		
:AsscociateProfessor rdf:type owl:Class ;
  rdfs:subClassOf :AcademicOffice ;
  rdfs:label "Außerordentlicher Professor"@de, "Associate Professor"@en ;
	rdfs:comment "Bezeichnet einen Professor, der eine außerordentliche Professur (aO) inne hat. Diese Professoren lehrten ohne Lehrstuhl. Die außerordentliche Professur war aber in der Regel mit Expektanz auf einen vakant werdenden Lehrstuhl verknüpft."@de, "Associate professors who taught without holding a chair. The associate professorship, however, was usually linked to an expectation of a chair that would become vacant."@en .	

:AuctionCatalogue rdf:type owl:Class ;
  rdfs:subClassOf :Publication ;
  rdfs:label "Auktionskatalog"@de, "Auction catalogue"@en ;
	dc:description "Bezieht sich auf Auktionskataloge von Professorenbibliotheken, die nach dem Tod von Professoren veräußert wurden. Diese Kataloge listen manchmal nicht nur den zu veräußernden bibliothekarischen Nachlass, sondern oft auch Objektsammlungen oder Mobiliar des Verstorbenen."@de, "Refers to auction catalogues of professors' libraries sold after the death of professors. These catalogues sometimes list not only the library estate to be sold, but often also object collections or furniture of the deceased."@en .		
		
:Baccalaureus rdf:type owl:Class ;
  rdfs:subClassOf :Graduation ;
  rdfs:label "Baccalaureus"@de, "Baccalaureus"@en ;
	rdfs:comment "Bezeichnet den akademischen Grad eines Baccalaren/Baccalaureus. Kürzel: Bacc."@de , "Refers to the academic degree of a bachelor/baccalaureus.  Abbreviation: Bacc."@en .
		
:Birth rdf:type owl:Class ;
  rdfs:subClassOf :StageOfLife ;
  rdfs:derivedFrom <http://purl.org/pcp-on-web/ontology#Birth> ;
  rdfs:label "Geburt"@de, "Birth"@en ;
	rdfs:comment "Geburtsdatum oder Zeitraum einer Person."@de, "Birthdate or the period of birth of a person."@en .

:Candidacy rdf:type owl:Class ;
  rdfs:subClassOf :StageOfLife ;
  rdfs:label "Kandidatur"@de, "Candidacy"@en ;
	rdfs:comment "Bezieht sich auf die Kandidatur einer Person, die im Zuge der Besetzung einer Professur als Kandidat gehandelt wird. Diese Person kann ein Kandidat ohne Lehrstuhl sein, aber auch ein bereits amtierender Professor, der für einen anderen Lehrstuhl gehandelt wird."@de , "Refers to the candidacy of a person which is a candidate for a university chair/professorship. This person can be a candidate without a chair, but also an incumbent professor who is being traded for another chair."@en .
		
:Chair rdf:type owl:Class ;
  rdfs:subClassOf :Faculty ;
  rdfs:label "Lehrstuhl"@de, "Chair"@en ;
	rdfs:comment "Bezeichnet einen Lehrstuhl an einer Universitätsfakultät, der ein spezifisches Fachgebiet umfasst und mit einer Professur besetzt ist."@de, "Designates a chair at a university faculty that covers a specific subject area and is occupied by a professorship."@en .

:Collection rdf:type owl:Class ;
  rdfs:subClassOf :StageOfLife ;
  rdfs:label "Sammlung"@de, "Collection"@en ;
	rdfs:comment "Objekt-Sammlungen eines Professors, z.B. Privatbibliotheken, Naturalien- und Instrumentensammlungen, Kunstsammlungen etc."@de, "Object-collections of a professor, e.g. private libraries, naturalia or further scholarly devices, as well as art collections."@en .
		
:Corporation rdf:type owl:Class ;
  rdfs:derivedFrom <http://purl.org/pcp-on-web/ontology#Body> ;
  rdfs:subClassOf dc:Agent ;
  rdfs:label "Körperschaft"@de, "Corporation"@en ;
	rdfs:comment "Bezeichnet eine Körperschaft, eine rechtsfähige Institution."@de, "Refers to a corporation or corporate body in the sense of a legal institution."@en .

:Curriculum rdf:type owl:Class ;
  rdfs:subClassOf :Document ;
  rdfs:label "Lektionskatalog"@de, "Curriculum"@en ;
	rdfs:comment "Lektions-/Vorlesungskatalog einer Universität."@de, "Curriculum or lecture catalogue of a university."@en .
	
:Denomination rdf:type owl:Class ;
  rdfs:subClassOf :StageOfLife ;
  rdfs:derivedFrom <http://purl.org/pcp-on-web/ontology#denomination> ;
  rdfs:label "Konfession"@de, "Denomination"@en ;
	rdfs:comment "Religionszugehörigkeit oder Glaubenbekenntnis einer Person."@de , "The religious denomination of a person."@en .
		
:Death rdf:type owl:Class ;
  rdfs:subClassOf :StageOfLife ;
  rdfs:derivedFrom <http://purl.org/pcp-on-web/ontology#Death> ;
  rdfs:label "Tod"@de, "Death"@en ;
	rdfs:comment "Sterbedatum oder Zeitraum des Todes einer Person."@de, "Day of death or the period of death of a person."@en .				     

:Dissertation rdf:type owl:Class ;
  rdfs:subClassOf :Publication ;
  rdfs:derivedFrom <http://purl.org/pcp-on-web/ontology#QualificationDocument> ;
  rdfs:label "Dissertation"@de, "Dissertation"@en ;
	rdfs:comment "Bezeichnet das gedruckte Medium der Disputation. Die Dissertation ist im frühneuzeitlichen Kontext dieser Domäne als Werbeschrift für die Disputation zu betrachten, die in Kürze jene relevanten Thesen zusammenfasste, welche während der Disputation verhandelt wurden."@de, "Refers to the printed media of a disputation. In the early modern context of this domain it functioned as advertisement of the disputation as practice which briefly summoned the thesises of the given topic."@en .
		
:Disputation rdf:type owl:Class ;
  rdfs:subClassOf :TeachingPractices;
  rdfs:label "Disputation"@de, "Disputation"@en ;
	rdfs:comment "Bezieht sich auf die Disputationspraxis, dem wissenschaftlichen Streitgespräch. Es diente dem Zweck der Übung, der Graduierung oder Lehrbefähigung (venia legendi) und verwies als Inauguraldisputation pro loco auf die Erlangung einer Professur. Die Dissertation ist das gedruckte Medium der Dispuation."@de, "Refers to the practice of disputation, a scientific debate which had the purpose of practising curricula, to obtain academic titles and the right to teach and give lectures (venia legendi). It also refers to inaugural disputations of newly vocated professors. The printed medium of a disputation is the dissertation."@en .
		
:Doctor rdf:type owl:Class ;
  rdfs:subClassOf :Graduation ;
  rdfs:derivedFrom <http://purl.org/pcp-on-web/ontology#GraduationDoctorate> ;
  rdfs:label "Doctor"@de, "Doctor"@en ;
	rdfs:comment "Bezeichnet den akademischen Grad eines Doktoren. Kürzel: Dr."@de , "Describes the academic degree of a doctor. Abbreviation: Dr."@en .

:Document rdf:type owl:Class ;
  rdfs:derivedFrom <http://purl.org/pcp-on-web/ontology#Document> ;
  rdfs:subClassOf <http://purl.org/spar/fabio/Expression> ;
  rdfs:subClassOf <http://purl.org/dc/terms/BibliographicResource> ;
  rdfs:label "Dokument"@de, "Document"@en ;
	rdfs:comment "Dokument unterschiedlicher Genres und Medien, die für die Lebensabschnitte eines Professors relevant sind."@de, "General Documents of different genres and media which are relevant for the stages of life of professors."@en .
		
:Education  rdf:type owl:Class ;
  rdfs:subClassOf :StageOfLife ;
  rdfs:label "Bildungsweg"@de, "Education"@en ;
	rdfs:comment "Beschreibt den Bildungsweg einer Person."@de , "Decribes the education of a person."@en .

:Enrollment rdf:type owl:Class ;
  rdfs:subClassOf :UniversityStudies ;
  rdfs:label "Immatrikulation"@de, "Enrollment"@en ;
	rdfs:comment "Bezieht sich auf die Einschreibung einer Person in das Universitätsverzeichnis, die (Universitäts-)Matrikel."@de, "Refers to the enrollment of a person into the universities' directory, the (university) 'Matrikel'."@en .

:Exercise rdf:type owl:Class ;
  rdfs:subClassOf :TeachingPractices;
  rdfs:label "Übung"@de, "Exercise"@en ;
	rdfs:comment "Bezieht sich auf die Lehr- und Lernpraktik einer Übung."@de, "Refers to the teaching and learning practice of an exercise."@en .
		
:Faculty rdf:type owl:Class ;
  rdfs:subClassOf :University ;
  rdfs:derivedFrom <http://purl.org/pcp-on-web/ontology#Faculty> ;
  rdfs:label "Fakultät"@de, "Faculty"@en ;
	rdfs:comment "Bezieht sich auf eine körperschaftlich organisierte und auf ein Fachgebiet begrenzte Lehr- und Verwaltungseinheit einer Volluniversität, im frühneuzeitlichen Kontext: Artistenfakultät (facultas artium), später Philosophische Fak., Theologie, Jurisprudenz, Medizin."@de, "Refers to corporated university divisions with specific subject areas, which are in an Early Modern context: facultas artium, later Philosophical fac., Theology, Jurisprudence, Medicine."@en .

:FacultyOfLaw rdf:type owl:Class ;
  rdfs:subClassOf :Faculty ;
  rdfs:label "Juristische Fakultät"@de, "Faculty of Law"@en ;
	rdfs:comment "Bezeichnet die Juristische Fakultät an einer Universität."@de, "Refers to the Faculty of Law at Universities."@en .
		
:FacultyOfMedicine rdf:type owl:Class ;
  rdfs:subClassOf :Faculty ;
  rdfs:label "Medizinische Fakultät"@de, "Faculty of Medicine"@en ;
	rdfs:comment "Bezeichnet die Medzinische Fakultät an einer Universität."@de, "Refers to the Faculty of Medicine at Universities."@en .
		
:FacultyOfPhilosophy rdf:type owl:Class ;
  rdfs:subClassOf :Faculty ;
  rdfs:label "Philosophische Fakultät"@de, "Faculty of Philosophy"@en ;
	rdfs:comment "Bezeichnet die Artesfakultät, die sich im Untersuchungszeitraum zu einer Philosophischen Fakultät entwickelte und an der propädeutisches Wissen für das weitergehende Studium an den übrigen höheren Fakultäten einer Volluniversität vermittelt wurde."@de, "Refers to the facultats artium which developed into a faculty of philosophy throughout the period of interest and at which propaedeutic knowledge was taught for further studies at one of the higher faculties of a full university."@en .
		
:FacultyOfTheology rdf:type owl:Class ;
  rdfs:subClassOf :Faculty ;
  rdfs:label "Theologische Fakultät"@de, "Faculty of Theology"@en ;
	rdfs:comment "Bezeichnet die Theologische Fakultät an einer Universität."@de, "Refers to the Faculty of Theology at Universities."@en .
		
:Family rdf:type owl:Class ;
  rdfs:subClassOf :StageOfLife ;
  rdfs:derivedFrom <http://purl.org/pcp-on-web/ontology#Family> ;
  rdfs:label "Familie"@de, "Family"@en ;
	rdfs:comment "Dieses Konzept beschreibt die soziale Herkunft und Familienverhältnisse einer Person."@de, "This concept describes the social origin and the family relationship of a person."@en .
		
:Graduation rdf:type owl:Class ;
  rdfs:subClassOf :StageOfLife ;
  rdfs:derivedFrom <http://purl.org/pcp-on-web/ontology#Graduation> ;
  rdfs:label "Abschluss"@de, "Graduation"@en ;
	rdfs:comment "Bezieht sich auf den Abschluss an einer Universität. Dieser kann durch eine Promotion zum Magister, Baccalaureus, Lizentiat, Doktor belegt sein, bspw. über eine pro gradu disputatio."@de, "Refers to a graduation at a university to the degrees of doctor, magister, baccalaureus, licentiate, e.g. proven via a pro gradu disputatio."@en .
		
:Honour rdf:type owl:Class ;
  rdfs:subClassOf :StageOfLife ;
  rdfs:derivedFrom <http://purl.org/pcp-on-web/ontology#Honour> ;
  rdfs:label "Ehrung"@de , "Honour"@en ;
	rdfs:comment "Dieses Konzept beschreibt eine Ehrung, wie wissenschaftliche Auszeichnungen oder Preise."@de, "This concept describes an honour, such as scientific awards or prizes."@en .
		
:Institution rdf:type owl:Class ;
  rdfs:subClassOf :Corporation ;
  rdfs:derivedFrom <http://purl.org/pcp-on-web/ontology#Institution> ;
  rdfs:label "Institution"@de , "Institution"@en ;
	rdfs:comment "In Abgrenzung zur Körperschaft ist die Institution hier eine Einrichtung ohne Rechtscharakter."@de, "In distinction to a coropration refers this concept to institutions without legal power."@en .
		
:Keyword rdf:type owl:Class ;
  rdfs:label "Schlagwort"@de, "Keyword"@en ;
	rdfs:comment "Zusätzliche Informationen, die in den Datenbanken unter Schlagworten und Kommentarfunktionen verborgen sind und ganz unterschiedlicher Natur sein können."@de, "Additional information given under keyword or commentary in the original databases and which can be varied in content."@en . 
				
:Lecture rdf:type owl:Class ;
  rdfs:subClassOf :TeachingPractices ;
  rdfs:derivedFrom <http://purl.org/pcp-on-web/ontology#Lecture> ;
  rdfs:label "Vorlesung"@de, "Lecture"@en ;
	rdfs:comment "Bezieht sich auf Vorlesungen bzw. Lektionen (lectiones), die von einem Professor im Rahmen der universitären Lehre in Vorlesungsverzeichnissen angekündigt wurden."@de, "Refers to lectures announced by a professor in the curriculum of a university."@en .

:Lecturer rdf:type owl:Class ;
  rdfs:subClassOf :AcademicOffice ;
  rdfs:label "Privatdozent"@de, "Lecturer"@en ;
	rdfs:comment "Bezeichnet Lehrkräfte ohne Professur, oft als PD bezeichnet. Graduierte Personen wie Magister oder Doktoren, die mit Lehrbefähigung (venia legendi/docendi) an der Universität lehrten, aber kein regelmäßiges Salär über die Korporation bzw. die Landesherrschaft erhielten. Stattdessen bekamen sie direkt von den Studenten Honorare für ihre Lehrpraxis."@de, "Refers to teachers without professorships but the permission to teach (venia legendi/docendi), often referred to as PD. Those were graduated persons, such as Magister or Doctors who did not receive a salary by the corporation or territory ruler but got paid directly by the students for their teaching practices."@en .
			
:LectureDone rdf:type owl:Class ;
  rdfs:subClassOf :Lecture ;
  rdfs:label "abgehaltene Vorlesung"@de, "Lecture done"@en ;
	rdfs:comment "Bezieht sich auf Vorlesungen (lectiones) die von Professoren nachweislich durchgeführt wurden, z.B. nachgewiesen in Rechenschaftsberichten oder aktenkundliche Lektionslisten."@de, "Refers to lectures which were actually given by a professor and which can be proved to be given, e.g. by reports, lists or other archival material."@en .	
		
:Licentiatus rdf:type owl:Class ;
  rdfs:subClassOf :Graduation ;
  rdfs:label "Lizenziat"@de, "Licentiate"@en ;
	rdfs:comment "Bezeichnet den akademischen Grad eines Lizenziaten, eines Baccalaren mit Lehrbefugnis. Zugleich einen Doktor der evang. Theologie (bis 1947 an deutschen Hochschulen). Kürzel: lic."@de , "Describes the academic degree of a Licentiate, which means a bachelor/baccalaureus with the right to teach. Also the academic title of a doctor of Evangelic theology (valid until 1947 in Germany). Abbreviation: lic."@en .
		
:Location rdf:type owl:Class ;
  rdfs:subClassOf wgs84:SpatialThing;	
  rdfs:label "Ort"@de, "Location"@en ;
	rdfs:comment "Bezieht sich auf den geografischen Ort für Lebensabschnitte einer Person, Orte von Körperschaften, Medien (Verlagsort, Druckort), Ämtern, Landesherrschaft usw."@de, "Refers to the geographical location of life stages of persons, corporate bodies, media (printing, publishing), offices, territories and others."@en .

:Magister rdf:type owl:Class ;
  rdfs:subClassOf :Graduation ;
  rdfs:label "Magister"@de, "Magister"@en ;
	rdfs:comment "Bezeichnet den akademischen Grad eines Magister. Kürzel: Mag."@de , "Refers to the academic degree of a Magister. Abbreviation: Mag."@en .

:Membership rdf:type owl:Class ;
  rdfs:subClassOf :StageOfLife ;
  rdfs:derivedFrom <http://purl.org/pcp-on-web/ontology#Membership> ;
  rdfs:label "Mitgliedschaft"@de, "Membership"@en ;
	rdfs:comment "Verweist auf Mitgliedschaften einer Person in soziokulturellen und/oder politischen Gesellschaften, Sozietäten und weiterer Institutionen; auch Studentenverbindungen."@de, "Refers to the membership of a person at sociocultural and/or political societies or further institutions; also fraternities."@en .
		
:Office rdf:type owl:Class ;
  rdfs:subClassOf :StageOfLife;
  rdfs:derivedFrom <http://purl.org/pcp-on-web/ontology#Office> ;
  rdfs:label "Amt"@de, "Office"@en ;
	rdfs:comment "Bezieht sich auf nicht akademische Ämter bzw. Nebenberufe von Professoren außerhalb der Universität, z.B. als Ärzte, Räte oder Anwälte."@de , "Refers to non-academic offices resp. side professions of professors outside of the university, e.g. as physicians at court, lawyers or counselers."@en .

:Pamphlet rdf:type owl:Class ;
  rdfs:subClassOf :Publication ;
  rdfs:label "Streitschrift"@de, "Pamphlet"@en ;
	rdfs:comment "Bezeichnet eine Streitschrift."@de, "Refers to a pamphlet."@en .
			
:Person rdf:type owl:Class ;
  rdfs:derivedFrom <http://purl.org/pcp-on-web/ontology#Person> ;
  rdfs:subClassOf dc:Agent ;
  rdf:label "Person"@de, "Person"@en ;
	rdfs:comment "Bezeichnet eine Person."@de, "Refers to a person."@en .
		
:Picture rdf:type owl:Class ;
  rdfs:subClassOf :StageOfLife ;		
  rdfs:derivedFrom <http://purl.org/pcp-on-web/ontology#Picture> ;
  rdfs:label "Bild"@de, "Picture"@en ;
	rdfs:comment "Dieses Konzept beschreibt das Bild einer Person."@de, "This concept describes the picture of a person."@en .
		
:PrimaryEducation  rdf:type owl:Class ;
  rdfs:subClassOf :Education ;
  rdfs:label "Primäre Bildung"@de, "Primary education"@en ;
	rdfs:comment "Bezieht sich auf die diversen vormodernen Schulformen und pädagogischen Bildungsangebote im Vorfeld eines Universitätsbesuchs im Territorium des Heiligen Römischen Reichs Deutscher Nation, z.B. Elementarschulen, Lateinschulen, Gymnasien, Klosterschulen, Pfarrschulen etc."@de , "Refers to the diverse early modern educational and pedagogical formas and institutions of primary education within the Holy Roman Empire."@en .		

:PrivateLibrary rdf:type owl:Class ;
  rdfs:subClassOf :Collection ;
  rdfs:label "Privatbibliothek"@de, "Private library"@en ;
	dc:description "Verweist auf die Privatbibliothek einer Person und kann u.U. durch publizierte Auktionskataloge erschlossen werden."@de, 
		"Refers to the private library of a person. Can be reconstructed by published auction catalogues."@en .		
			
:PrivateEducation rdf:type owl:Class ;
  rdfs:subClassOf :Education ;
  rdfs:label "Privatunterricht"@de, "Private education"@en ;
	rdfs:comment "Privatunterricht im Familienverband oder durch einen Privatlehrer."@de,
		"Private education by family members or a different private teacher."@en .
		
:PrivateLecture rdf:type owl:Class ;
  rdfs:subClassOf :Lecture;
  rdfs:label "Private Vorlesung"@de, "Private Lecture"@en ;
	rdfs:comment "Bezieht sich auf private Vorlesungen (lectio privata, privatum, privatissimum), die ein Professor in einem kleinen Kreis von Studenten hält und die von den Studenten in der Regel an den Professor selbst bezahlt werden mussten."@de, "Refers to private lectures (lectio privata, privatum, privatissimum), given by a professor for a relatively small amount of students, which a 	student usually had to pay for directly to the Professor."@en .
		
:Professor rdf:type owl:Class ;
  rdfs:subClassOf :Person ;
  rdfs:derivedFrom <http://purl.org/pcp-on-web/ontology#Professor> ;
  rdfs:label "Professor"@de, "Professor"@en ;
	rdfs:comment "Bezeichnet ordentliche Professoren an frühneuzeitlichen Universitäten im deutschsprachigen Raum des Heiligen Römischen Reichs, deren Karrierewege im Fokus des für die Ontologie maßgebenden Forschungsprojektes liegen."@de,
		"Refers to full or ordinary professors at early modern universities in the German-speaking area of the Holy Roman Empire whose career paths are the focus of the research project relevant to the given ontology."@en .

:ProfessorialFamily rdf:type owl:Class ;
  rdfs:subClassOf :Family ;
  rdfs:label "Professorenfamilie"@de, "Professorial Family"@en ;
	rdfs:comment "Bezieht sich auf Familien die generationenübegreifend auffallend häufig Professoren hervorbrachten. Diese Familien werde in der Forschung häufig mit Begriffen wie Gelehrtendynastie und Familienuniversität belegt."@de, "Refers to families that produced professors with a striking frequency across the generations. In research, these families are often referred to by terms such as scholarly dynasty and family university."@en . 
		
:Professorship rdf:type owl:Class ;
  rdfs:subClassOf :AcademicOffice ;
  rdfs:label "Professur"@de, "Professorship"@en ;
	rdfs:comment "Bezeichnet den Lehrstuhl eines ordentlichen Professors an einer Universitätsfakultät, der einem Fachgebiet zugeordnet ist."@de, "Designates the chair of a full or ordinary Professor at a university faculty."@en .
		
:ProgramsAndSpeeches rdf:type owl:Class ;
  rdfs:subClassOf :Publication ;
  rdfs:label "Programme und Reden"@de, "Programs and Speeches"@en ;
	rdfs:comment "Bezieht sich auf gedruckte Universitätsprogramme und Reden."@de, "Refers to printed university programs and speeches."@en .

:Publication rdf:type owl:Class ;
  rdfs:subClassOf :Document ;	
  rdfs:derivedFrom <http://purl.org/pcp-on-web/ontology#Publication> ;
  rdfs:label "Publikation"@de, "Publication"@en ;
	rdfs:comment "Bezieht sich auf Publikationen."@de, "Refers to publications."@en .

:Publicist rdf:type owl:Class ;
  rdfs:subClassOf :StageOfLife;
  rdfs:label "Publizist"@de, "Publicist"@en ;
	rdfs:comment "Bezieht sich auf den Lebensabschnitt eines Professors als Publizist, d. h. als Autor oder Herausgeber auf dem zeitgenössischen Publikationsmarkt auftritt."@de, "Refers to the stage of a professor's life as a publicist, appearing as an author or editor on the contemporary publication market."@en .		
		
:PublicLecture rdf:type owl:Class ;
  rdfs:subClassOf :Lecture ;
  rdfs:label "Öffentliche Vorlesung"@de, "Public Lecture"@en ;
	rdfs:comment "Bezieht sich auf öffentliche Vorlesungen (lectio publica) von Professoren, die nicht extra vom Studenten bezahlt werden mussten."@de, 
		"Refers to public lectures (lectio publica) of professors which had not to be payed extra by students."@en .
		
:Recommendation  rdf:type owl:Class ;
  rdfs:subClassOf :StageOfLife ;
  rdfs:label "Empfehlung"@de, "Recommendation"@en ;
  	rdfs:comment "Bezieht sich auf Empfehlungen, z.B. Empfehlungsschreiben, die in Bestallungsakten enthalten sind."@de , "Refers to recommendations, e.g. letters of recommendation which are part of vocation files."@en .

:Report rdf:type owl:Class ;
  rdfs:subClassOf :Document ;
  rdfs:label "Rechenschaftsbericht"@de, "Report"@en ;
	rdfs:comment "Rechenschaftsbericht den Dozenten in regelmäßigen Abständen bei der Universitätverwaltung und Landesverwaltung einreichten."@de,
		"Means regular reports of lecturers about their curriculum to the university and territorial administration."@en .

:Review rdf:type owl:Class ;
  rdfs:subClassOf :Publication ;
  rdfs:label "Rezension"@de, "Review"@en ;
	rdfs:comment "Bezeichnet die Rezension in einer Rezensionszeitschrift."@de, "Refers to a review published in a review journal."@en .

:School rdf:type owl:Class ;
  rdfs:subClassOf :Institution ;
  rdfs:derivedFrom <http://purl.org/pcp-on-web/ontology#School> ;
  rdfs:label "Schule"@de, "School"@en ;
	rdfs:comment "Bezeichnet Schulen für die primäre Bildung."@de, "Refers to schools for primary education."@en .
			
:Semester rdf:type owl:Class ;
  rdfs:subClassOf :University ;
  rdfs:label "Semester"@de, "Semester"@en ;
    rdfs:comment "Abschnitt des Akademischen Jahrs. Es besteht aus einem Sommer- und einem Wintersemester."@de ,
		"Part of an academic year. It consists of a summer- and a wintersemester"@en .
		
:Seminar rdf:type owl:Class ;
  rdfs:subClassOf :TeachingPractices ;
  rdfs:label "Seminar"@de, "Seminar"@en ;
    rdfs:comment "Bezieht sich auf die Lehrveranstaltung eines Seminars, in den Quellen wie im Fall Uni Helmstedt mit Seminarium bezeichnet."@de ,"Refers to the course of a seminar, referred to in the sources as Seminarium, as in the case of the University of Helmstedt."@en .	
		
:Societies rdf:type owl:Class ;
  rdfs:subClassOf :Institution ;
  rdfs:derivedFrom <http://purl.org/pcp-on-web/ontology#AcademicSociety> ;
  rdfs:label "Gesellschaften"@de, "Societies"@en ;
	rdfs:comment "Bezeichnet Gesellschaften, wie Gelehrtengesellschaften, die sich einer bestimmten Geistesströmung oder Disziplin widmeten und aus Gelehrten und Gebildeten bestand sowie zumeist regional begrenzt agierte. Mit Gesellschaften konnten auch literarische Salons oder Lesegesellschaften gemeint sein. Außerdem Sozietäten mit strukturierter Körperschaft und obrigkeitlicher Protégierung (z.B. Akademie der Wissenschaften in Berlin). Des Weiteren sind mit Gesellschaften unter Umständen auch Geheimgesellschaften wie Freimaurer oder Illuminaten gemeint."@de, "Refers to societies like Learned Societies, which usually dealt with a certain discipline or ideas and which gathered learned and educated people, mostly of regionaly importance. Societies could also refer to literary salons or reading societies. Furthermore, societies with structured corporate body and most commonly protection and financing by the territory ruler, like the Akademie der Wissenschaften in Berlin. Furthermore societies could also refer to secret societies like Freemasons or Illuminati."@en .

:StageOfLife rdf:type owl:Class ;
  rdfs:derivedFrom <http://purl.org/pcp-on-web/ontology#PeriodOfLife> ;
  rdfs:label "Lebensabschnitt"@de, "Stage of Life"@en ;
	rdfs:comment "Dieses Konzept bezieht sich auf einen Lebensabschnitt eines Professors."@de, "This concept refers to a stage of life of a professor."@en .
		
:Statutes rdf:type owl:Class ;
  rdfs:subClassOf :University ;
  rdfs:label "Statuten"@de, "Statutes"@en ;
	rdfs:comment "Die Verfassung einer Universität."@de, "University constitution."@en .

:Student rdf:type owl:Class ;
  rdfs:subClassOf :Person ;
  rdfs:label "Student"@de, "Student"@en ;
	rdfs:comment "Bezeichnet einen an der Universität immatrikulierten Studenten."@de, "Refers to an enrolled student at a University."@en .
		
:SummerSemester rdf:type owl:Class ;
  rdfs:subClassOf :Semester ;
  owl:DisjoinUnionOf :WinterSemester;
  rdfs:label "Sommersemester"@de, "Summer Semester"@en ;
    rdfs:comment "Das halbjährige Sommersemester dauert von April bis September."@de , "The biannual summer semester starts in April and ends in September."@en .

:TeachingPractices rdf:type owl:Class ;
  rdfs:subClassOf :StageOfLife ;
  rdfs:label "Lehrpraktiken"@de, "Teaching Practices"@en ;
  	rdfs:comment "Beschreibt akademische Lehrpraktiken, die ein Professor an der Universität durchführt und welche durch Statuten, weitere Regularien und/oder durch Gewohnheit geregelt sind."@de, "Describes academic teaching practices which are regulated by the University's statutes or further regulations and/or customs."@en .
		
:Territory rdf:type owl:Class ;
  rdfs:subClassOf :Corporation ;
  rdfs:label "Landesherrschaft"@de, "Territory"@en ;
	rdfs:comment "Bezeichnet die Landesherrschaft eines Territoriums und bezieht sich hier auf den Amtssitz jener landesherrschaftlichen Organe, denen die Universitäten unterstellt sind."@de, "Refers to the authority by a ruler/rulership of a territory and means the territorial administration which deal with the universities."@en .

:Textbook rdf:type owl:Class ;
  rdfs:subClassOf :Publication ;
  rdfs:label "Lehrbuch"@de, "Textbook"@en ;
	rdfs:comment "Bezeichnet ein Buch das Lehrinhalte eines Studiums didaktisch aufbereitet."@de, "Refers to books which offer a compilation of content in a certain field of interest."@en .
		
:University rdf:type owl:Class ;
  rdfs:subClassOf :Corporation ;
  rdfs:derivedFrom <http://purl.org/pcp-on-web/ontology#Academy> ;
  rdfs:label "Universität"@de, "University"@en ;
	rdfs:comment "Bezeichnet eine Lehr-, Bildungs- und Forschungskorporation die dazu priviligiert ist, akademische Grade zu verleihen."@de ,
		"Refers to education and research corporations which own the privilige to award academic degrees."@en .
				     
:UniversityStudies rdf:type owl:Class ;
  rdfs:subClassOf :Education ;
  rdfs:derivedFrom <http://purl.org/pcp-on-web/ontology#Study> ;
  rdfs:label "Studium"@de, "University studies"@en ;
	rdfs:comment "Bezieht sich auf das Universitätsstudium einer Person."@de, "Refers to the university studies of a person."@en .

:WinterSemester rdf:type owl:Class ;
  rdfs:subClassOf :Semester ;
  owl:DisjoinUnionOf :SummerSemester;
  rdfs:label "Wintersemester"@de, "Winter Semester"@en ;
    rdfs:comment "Das halbjährige Wintersemester dauert von Oktober bis März."@de , "The biannual winter semester starts in October and ends in March."@en .		

#################################################################
#		Datatype Propertys		
#################################################################
	
:academicYear rdf:type owl:DatatypeProperty ;
  rdfs:domain :Semester ;
  rdfs:range xsd:gYear;
  rdfs:label "Academic Year"@en, "Akademisches Jahr"@de .

###  http://purl.org/pcp-on-web/ontology#additionToSurname
:additionToSurname rdf:type owl:DatatypeProperty ,
                            owl:FunctionalProperty ;
                   rdfs:domain :Person ;
                   rdfs:range xsd:string ;
                   rdfs:comment "Additions to the surname can be of, etc."@en ,
                                "Namenszusätze sind zum Beispiel von, zu, etc."@de ;
                   rdfs:label "additions to surname"@en ,
                              "Namenszusatz"@de ;
                   owl:versionInfo "0.2 changed Domain from Professor to Person 0.1 initial creation - 24.05.07"^^xsd:string ,
                                   "2.0 stable"^^xsd:string .


###  http://purl.org/pcp-on-web/ontology#alternativeWritingOfSurname
:alternativeWritingOfSurname rdf:type owl:DatatypeProperty ,
                                      owl:FunctionalProperty ;
                             rdfs:domain :Person ;
                             rdfs:range xsd:string ;
                             <http://ns.ontowiki.net/SysOnt/order> "20"^^xsd:string ;
                             rdfs:comment "Bsp: Meier, Meyer, Maier"@de ,
                                          "For Example Meier, Meyer, Maier"@en ;
                             rdfs:label "alternative Namensschreibweisen"@de ,
                                        "alternative writings of the surname"@en ;
                             owl:versionInfo "0.1 initial creation - 24.05.07"^^xsd:string ,
                                             "0.2 changed Domain from Professor to Person"^^xsd:string ,
                                             "2.0 under discussion"^^xsd:string .


:date rdf:type owl:DatatypeProperty, owl:FunctionalProperty ;
  rdfs:domain :StageOfLife ;
  rdfs:range rdfs:Literal;
  rdfs:label "Date"@en, "Datum"@de ;
  	rdfs:comment """Zeitangabe eines Lebensabschnitts."@de, "The date or timespan of a stage of life from a valid datatype
		 xsd:date ,
                 xsd:gDay ,
                 xsd:gMonth ,
                 xsd:gMonthDay ,
                 xsd:gYear ,
                 xsd:gYearMonth"""@en .
				     
:docDate rdf:type owl:DatatypeProperty, owl:FunctionalProperty ;
  rdfs:domain :Document ;
  rdfs:range rdfs:Literal;
  rdfs:label "Date Document"@en, "Datum Dokument"@de ;
  	rdfs:comment """Zeitangabe eines Dokuments, z.B. Veröffentlichungsjahr, Datum eines Rechenschaftsberichts etc. ."@de, "The date or timespan of a document from a valid datatype, like publishing years or the given date of a report etc.
		 xsd:date ,
                 xsd:gDay ,
                 xsd:gMonth ,
                 xsd:gMonthDay ,
                 xsd:gYear ,
                 xsd:gYearMonth"""@en .
				     
:enrollmentSemester rdf:type owl:DatatypeProperty ;
  rdfs:domain :Enrollment ;
  rdfs:range :Semester ;
  rdfs:label "Semester der Immatrikulation"@de, "semester of enrollment"@en ;
	rdfs:comment "Nennt das Semester der Immatrikulation eines Professors."@de, "Gives information of the semester in which a person got enrolled."@en .
				     
###  http://purl.org/pcp-on-web/ontology#forename
:forename rdf:type owl:DatatypeProperty ;
          rdfs:domain :Person ;
          rdfs:range rdfs:Literal;
          rdfs:comment "Forename(s) of a person, seperated by space"@en ,
                       "Vorname(n) einer Person, getrennt mit Leerzeichen"@de ;
          rdfs:label "Forename"@en ,
                     "Vorname"@de ;
          owl:versionInfo "0.1 initial creation date: 18.05.2015"^^xsd:string .

###  http://purl.org/pcp-on-web/ontology#from
:from rdf:type owl:DatatypeProperty ;
      rdfs:domain :StageOfLife ;
      rdfs:range rdfs:Literal ;
      rdfs:comment "Das Startdatum eines Lebensabschnitts"@de ,
                   """The date of the beginning of a stage of life from a valid datatype xsd:date ,
                 xsd:gDay ,
                 xsd:gMonth ,
                 xsd:gMonthDay ,
                 xsd:gYear ,
                 xsd:gYearMonth"""@en ;
      rdfs:label "from"@en ,
                 "von"@de ;
      owl:versionInfo "0.1 initial creation date:  24.05.2007"^^xsd:string ,
                      "2.0 stable other types added"^^xsd:string .
				     
###  http://purl.org/pcp-on-web/ontology#furtherInformation
:furtherInformation rdf:type owl:DatatypeProperty ,
                             owl:FunctionalProperty ;
                    rdfs:domain :Person ;
                    rdfs:range rdfs:Literal ;
                    <http://ns.ontowiki.net/SysOnt/order> "340"^^xsd:string ;
                    rdfs:label "further information"@en ,
                               "weitere Informationen"@de ;
                    owl:versionInfo "0.1 initial creation - 28.06.2007"^^xsd:string ,
                                    "2.0 stable"^^xsd:string .

:gender rdf:type owl:DatatypeProperty ;
  rdfs:domain :Person ;
  rdfs:derivedFrom <http://purl.org/pcp-on-web/ontology#gender> ;
  rdfs:label "Geschlecht"@de, "Gender"@en ;
	rdfs:comment "Verweist auf das biologische Geschlecht oder die Geschlechtsidentität einer Person."@de, "Refers to sex or gender of a person."@en .
			    
:gnd rdf:type owl:DatatypeProperty , owl:FunctionalProperty ;
  rdfs:domain :Person ;
  rdfs:range rdfs:Literal ;
  rdfs:label "GND"@de, "GND"@en ;
  	rdfs:comment "GND Normadatei, inklusive ehemals genutzte PND."@de, "GND integrated authority file, including formerly used PND."@en .
				     
:latinForename rdf:type owl:DatatypeProperty ;
                   rdfs:domain :Person ;
				   rdfs:range rdfs:Literal ;
                   rdfs:comment "Latinized first name of a person."@en ,
                                "Latinisierter  Vorname einer Person."@de ;
                   rdfs:label "Latin First Name"@en ,
                              "Latinisierter Vorname"@de ;
                   owl:versionInfo "PCP-on-Web 1 including property from merging Helmstedt data - 27.06.18"^^xsd:string .

:latinSurname rdf:type owl:DatatypeProperty ;
                   rdfs:domain :Person ;
				   rdfs:range rdfs:Literal ;
                   rdfs:comment "Latinized last name of a person."@en ,
                                "Latinisierter Nachname einer Person."@de ;
                  rdfs:label "Latin Last Name"@en ,
                              "Latein Name"@de ;
                   owl:versionInfo "PCP-on-Web 1 including property from merging Helmstedt data - 27.06.18"^^xsd:string .
				     
:locationCorporation rdf:type owl:DatatypeProperty ;
  rdfs:domain :Corporation ;
  rdfs:range :Location ;
  rdfs:derivedFrom <http://purl.org/pcp-on-web/ontology#bodyPlace> ;
  rdfs:label "Ort einer Körperschaft"@de, "location of a corporation"@en ;
	rdfs:comment "Bezieht sich auf den geografischen Ort einer Körperschaft."@de,
		"Refers to the geographical location of a corporation."@en .

:locationDocument rdf:type owl:DatatypeProperty ;
  rdfs:domain :Document ;
  rdfs:range :Location ;
  rdfs:label "Ort eines Dokument"@de, "location of a document"@en ;
	rdfs:comment "Bezieht sich auf den geografischen Ort eines Dokuments, z.B. Publikationsort."@de,
		"Refers to the geographical location of a document, e.g. location of a publication."@en .

###  http://purl.org/pcp-on-web/ontology#note
:note rdf:type owl:DatatypeProperty ,
               owl:FunctionalProperty ;
      rdfs:domain :Person ;
      rdfs:range rdfs:Literal ;
      <http://ns.ontowiki.net/SysOnt/order> "390"^^xsd:string ;
      rdfs:comment "additional information that does not fit elsewhere"@en ,
                   "zusätzliche Informationen die nirgends sonst eingetragen werden können"@de ;
      rdfs:label "Vermerk, Hinweis"@de ,
                 "note"@en ;
      owl:versionInfo "0.1 initial creation - 24.05.2007"^^xsd:string ,
                      "0.2 changed Domain from Professor to Person"^^xsd:string ,
                      "2.0 stable"^^xsd:string .
	      
:pagination rdf:type owl:DatatypeProperty ;
                   rdfs:domain :Document ;
				   rdfs:range rdfs:Literal ;
                   rdfs:comment "Pagination of a document."@en ,
                                "Seitennummerierung eines Dokuments"@de ;
                   rdfs:label "Pagination"@en ,
                              "Seitennummerierung"@de ;
                   owl:versionInfo "PCP-on-Web 1 including property from merging Helmstedt data - 27.06.18"^^xsd:string .
	      
:pid rdf:type owl:DatatypeProperty ;
                   rdfs:domain :Person ;
				   rdfs:range rdfs:Literal ;
                   rdfs:comment "Persons Identification number in the original database, including professors."@en ,
                                "Personen Identifikationsnummer in der ursprünglichen Datenbank, inkl. Professoren."@de ;
                   rdfs:label "PID"@en ,
                              "PID"@de ;
                   owl:versionInfo "PCP-on-Web 1 including property from merging Helmstedt data - 27.06.18"^^xsd:string .
				     
###  http://purl.org/pcp-on-web/ontology#surname
:surname rdf:type owl:DatatypeProperty ;
  rdfs:domain :Person ;
  rdfs:range rdfs:Literal ;
  rdfs:label "Nachname"@de , "surname"@en ;
  rdfs:comment "Nachname einer Person"@de , "The surname of a person"@en ;
		         owl:versionInfo "0.1 initial creation date: 24.05.2007"^^xsd:string ,
                         "2.0 stable"^^xsd:string ,
                         "version 0.2  10.03.2008"^^xsd:string .

:title rdf:type owl:DatatypeProperty ;
  rdfs:subPropertyOf <http://purl.org/dc/terms/title> ;
  rdfs:domain :Document ;
  rdfs:range xsd:literal ;
  rdfs:label "Titel eines Dokuments"@de, "title of a document"@en ;
	rdfs:comment "Nennt den Titel eines Dokuments."@de, "Gives the title of a document."@en .	      
	      
###  http://purl.org/pcp-on-web/ontology#to
:to rdf:type owl:DatatypeProperty ;
    rdfs:domain :StageOfLife ;
    rdfs:range rdfs:Literal ;
    rdfs:comment "Das Enddatum eines Lebensabschnitts"@de ,
                 """The date of the ending of a stage of life from a valid datatype xsd:date ,
               xsd:gDay,
               xsd:gMonth,
               xsd:gMonthDay,
               xsd:gYear,
               xsd:gYearMonth"""@en ;
    rdfs:label "bis"@de ,
               "to"@en ;
    owl:versionInfo "0.1 initial creation date:  24.05.2007"^^xsd:string ,
                    "2.0 stable other types added"^^xsd:string .
				     
#####################################################################################################################################################################
#				     Object Properties				     
#####################################################################################################################################################################    
				     
:author rdf:type owl:ObjectProperty ;
  rdfs:subPropertyOf dc:creator;
  rdfs:domain :Person, :Corporation ;
  rdfs:range :Document ;
  rdfs:derivedFrom <http://purl.org/pcp-on-web/ontology#hasTutor>, <http://purl.org/pcp-on-web/ontology#author>, <http://purl.org/pcp-on-web/ontology#published>, <https://d-nb.info/standards/elementset/gnd#author> ;
  rdfs:label "ist Autor"@de, "is author"@en ;
	rdfs:comment "Verweist auf die Autorenschaft eines Dokuments."@de, "Refers to the authorship of a document."@en .
	      
:child rdf:type owl:ObjectProperty ;
  rdfs:domain :Family ;  
  rdfs:range :Professor ;
  rdfs:derivedFrom <http://purl.org/pcp-on-web/ontology#familyChild> ;
  rdfs:label "Kind"@de, "child"@en ;
	rdfs:comment "Bezieht sich auf das Kind, Pflegekind, Adoptivkind eines Professors."@de, "Refers to the cild, foster child, adoptive child of a professor."@en .
	      
:correspondence rdf:type owl:ObjectProperty ;
  rdfs:subPropertyOf foaf:knows ;
  rdfs:domain :Person ;
  rdfs:range :Person ;
  rdfs:label "Korrespondenz"@de, "correspondence"@en ;
	rdfs:comment "Verweist auf die aus einem Dokument hervorgehende Korrespondenz zwischen Personen, z.B. über Editionen oder Nachlassplattformen wie KALLIOPE."@de, "Assigns to the correspondence between persons, e.g. via editions or heritage plattforms such as KALLIOPE."@en .

:dedicatee rdf:type owl:ObjectProperty ;
  rdfs:domain :Dissertation ;
  rdfs:range :Person ;
  rdfs:label "hat Widmungsempfänger"@de, "has dedicatee"@en ;
	rdfs:comment "Bezeichnet den Widmunsgempfänger einer Publikation."@de, "Refers to the dedicatee of a publication."@en .	      
	      
:dissertationHasDisputation rdf:type owl:ObjectProperty ;
  rdfs:domain :Dissertation ;
  rdfs:range :Disputation ;
  rdfs:label "Dissertation hat Disputation"@de, "dissertation has disputation"@en ;
	rdfs:comment "Weist eine Dissertation einer Disputation zu."@de, "Assigns a dissertation to a disputation."@en .

:dissHasFaculty rdf:type owl:ObjectProperty ;
  rdfs:domain :Dissertation ;
  rdfs:range :Faculty ;
  rdfs:label "Diss hat Fakultät"@de, "diss has faculty"@en ;
	rdfs:comment "Weist eine Dissertation einer Fakultät zu."@de, "Assigns a dissertation to a faculty."@en .
	      
:enrollmentName rdf:type owl:ObjectProperty ;
  rdfs:domain :Enrollment ;
  rdfs:range :Student ;
  rdfs:label "Name in Matrikel"@de, "name in enrollment document"@en ;
	rdfs:comment "Zumeist latinisierter Name eines Studenten im Matrikelbuch einer Universität."@de, "Most likely latinized name of a student at the enrollment document of a university."@en .
	      
:enrollmentOrigin rdf:type owl:ObjectProperty ;
  rdfs:domain :Enrollment ;
  rdfs:range :Location ;
  rdfs:label "Herkunft in Matrikel"@de, "origin in enrollment document"@en ;
	rdfs:comment "Zumeist latinisierter Herkunftsort eines Studenten im Matrikelbuch einer Universität."@de, "Most likely latinized name of origin of a student at the enrollment document of a university."@en .
	      
:geoname rdf:type owl:ObjectProperty ;
  rdfs:domain rdfs:Resource ;
  rdfs:range rdfs:Resource ;
  rdfs:derivedFrom <http://purl.org/pcp-on-web/ontology#geoname> ;
  rdfs:label "Geoname"@en , "Geoname"@de ;
  	rdfs:comment "The Resource location's URL in http://geonames.org."@en ,"Die URL des Ressourcenstandorts in http://geonames.org."@de; owl:versionInfo "PCP-on-Web 1 including property from merging Helmstedt data - 27.06.18"^^xsd:string .

:hasCreator rdf:type owl:ObjectProperty ;
  rdfs:subPropertyOf dc:creator;	      
  rdfs:domain :Document ;
  rdfs:range :Corporation, :Person ;
  rdfs:label "hat Urheber"@de, "has creator"@en ;
	rdfs:comment "Urheber eines Dokuments"@de, "Creator of a document."@en .	      
	      
:hasEnrollment rdf:type owl:ObjectProperty ;
  rdfs:domain :Student ;
  rdfs:range :Enrollment ;
  rdfs:derivedFrom <http://purl.org/pcp-on-web/ontology#hasEnrollment> ;  
  rdfs:label "hat Matrikel"@de, "has enrollment"@en ;
	rdfs:comment "Verweist auf eine Immatrikulation einer Person an einer Universität."@de, "Refers to the enrollment of a person at a university."@en .

:hasAuctionCatalogue rdf:type owl:ObjectProperty ;
  rdfs:domain :PrivateLibrary ;
  rdfs:range :AuctionCatalogue ;
  rdfs:label "hat Auktionskatalog"@de, "has auction catalogue"@en ;
	dc:description "Verknüpft eine Privatbibliothek mit einem Auktionskatalog."@de, "Adds an auction catalogue to a private library."@en .	      
	          
:hasRecommendation rdf:type owl:ObjectProperty ;
  rdfs:domain :Candidacy ;
  rdfs:range :Recommendation ;
  rdfs:label "hat Empfehlung"@de, "has recommendation"@en ;
	rdfs:comment "Gibt an, ob ein Kandidat ein Empfehlungsschreiben hat."@de, "Refers to any given recommendation of a candidate."@en .

:hasSchool rdf:type owl:ObjectProperty ;
  rdfs:domain :PrimaryEducation ;
  rdfs:range :School ;
  rdfs:label "hat Schule"@de, "has school"@en ;
	rdfs:comment "Verweist auf die Institution an der primäre Bildung erworben wurde."@de, "Refers to the institution of primary education."@en .
	      
:hasSemester rdf:type owl:ObjectProperty ;
  rdfs:domain :UniversityStudies, :TeachingPractices ;
  rdfs:range :Semester ;
  rdfs:label "Semesterangabe eines Studiums"@de, "semesters of a university study"@en ;
    rdfs:comment "Nennt Semester eines Studiums."@de,"Gives the semester of a university study."@en .

:hasStageOfLife rdf:type owl:ObjectProperty ;
  rdfs:domain :Professor ;
  rdfs:range :StageOfLife ;
  rdfs:derivedFrom <http://purl.org/pcp-on-web/ontology#hasPeriod> ;
  rdfs:label "hat Lebensabschnitt"@de, "has stage of life"@en ;
	rdfs:comment "Lebensabschnitt eines Professors."@de, "Stage of life of a professor."@en .
				     
:isDoing rdf:type owl:ObjectProperty ;
  rdfs:domain :Professor ;
  rdfs:range :TeachingPractices ;
  rdfs:label "hält oder führt durch"@de, "does or gives"@en ;
	rdfs:comment "Bezieht sich auf Lehrpraktiken, die von einem Professor an einer Universität durchgeführt werden, z.B. Vorlesungen halten, Disputationen vorstehen oder Übungen geben."@de, "Refers to teaching practices which are done by a professor at a university, e.g. give lectures, preside over disputations or give excersizes."@en.
	      
:isVocated rdf:type owl:ObjectProperty ;
  rdfs:domain :Candidacy ;
  rdfs:range :Professor ;
  rdfs:label "wird ernannt"@de, "is vocated"@en ;
	rdfs:comment "Bezieht sich auf den von Universität und Landesherrschaft ausgewählten Kandidaten für eine Professur."@de, "Refers to the candidate for a professorship/or chair which had been negotiated by the university and the territorial authority."@en .

:lectureHasDocument rdf:type owl:ObjectProperty ;
  rdfs:domain :Lecture ;
  rdfs:range :Document ;
  rdfs:label "Vorlesung hat Dokument"@de, "lecture has document"@en ;
	rdfs:comment "Weist einer Vorlesung ein Dokument zu, wie Lektionskatalog, Textbuch oder Rechenschaftsbericht."@de, "Assigns a lecture to a document, like curriculum, textbook or report."@en .
				     
:lectureHasFaculty rdf:type owl:ObjectProperty ;
  rdfs:domain :Lecture ;
  rdfs:range :Faculty ;
  rdfs:label "Vorlesung hat Fakultät"@de, "lecture has faculty"@en ;
	rdfs:comment "Weist eine Vorlesung einer Fakultät zu."@de, "Assigns a lecture to a faculty."@en .
	      
:membershipSociety rdf:type owl:ObjectProperty ;
  rdfs:domain :Membership ;
  rdfs:range :Societies ;
  rdfs:label "Mitgliedschaft hat Institution"@de, "membership has institution"@en ;
	rdfs:comment "Weist die Mitgliedschaft einer Institution zu."@de, "Adds the membership to an institution."@en .
				     				     
:nominates rdf:type owl:ObjectProperty ;
  rdfs:domain :Faculty ;
  rdfs:range :Candidacy ;
  rdfs:label "nominiert"@de, "nominates"@en ;
	rdfs:comment "Bezieht sich auf Nominierungslisten einer Fakultät, die an die Verwaltung der Landesherrschaft erging und aus denen ein Kandidat durch die Landesherrschaft bestätigt wurde. Diese Listen liegen zumeist in zuständigen Archiven vor."@de,
	"Refers to nomination lists which were handed in  to the territorial administration by the faculties in  order to choose and to vocate a  candidate for a university chair. Those lists can be found in relevant archives."@en .			     

:opponent rdf:type owl:ObjectProperty ;
  rdfs:domain :Person ;
  rdfs:range :Disputation ;
  rdfs:label "ist Opponent"@de, "is Opponent"@en ;
	rdfs:comment "Bezeichnet den Opponenten einer Disputation. Opponenten sind auf Titelblättern der gedruckten Disputationsschrift in der Regel nicht angegeben und konnten aus Lehrkräften sowie Studenten gleichermaßen bestehen. Zur Vollständigkeit und auch weil nicht ausgeschlossen werden kann, dass diese Elemete einer Disputation nicht doch in Disputationsschriften verzeichnet sind, hier diese Property."@de, "Refers to the opponent of a disputation. Opponents are usually not indicated on title pages of printed disputation papers aka dissertations and could consist of teachers as well as students.For the sake of completeness and also because it cannot be ruled out that these elements of a disputation are not listed in dissertations, here this property."@en .

:owns rdf:type owl:ObjectProperty ;
  rdfs:domain :Professor ;
  rdfs:range :Collection ;
  rdfs:label "besitzt"@de, "owns"@en ;
	rdfs:comment "Verweist auf Sammlungen eines Professors, z.B. Privatbibliotheken, Münzen und anderweitige fachspezifische Sammlungen, die bspw. für eine Person im Berufungsverfahren auf eine Professur von Bedeutung gewesen sein könnten."@de, "Refers to a collection of a professor, like private libraries, coins and other subject specific collections, which could have been important for the vocation of a professorship."@en .
				     
:parent rdf:type owl:ObjectProperty ;
  rdfs:domain :Family ;
  rdfs:range :Professor ;
  rdfs:derivedFrom <http://purl.org/pcp-on-web/ontology#familyParent> ;
  rdfs:label "Elternteil"@de, "parent"@en ;
	rdfs:comment "Weist einen Professor als Elternteil aus."@de, "Depicts a professor as a parent."@en .
	      
:ppn rdf:type owl:ObjectProperty ;
                   rdfs:domain :Dissertation ;
				   rdfs:range rdfs:Resource ;
                   rdfs:comment "The PICA Production Number (PPN) of a record."@en ,
                                "Die PICA Produktionsnummer (PPN) eines Datensatzes."@de ;
	           rdfs:derivedFrom <http://purl.org/pcp-on-web/ontology#ppn> ;
                   rdfs:label "PICA Production Number (PPN)"@en ,
                              "PICA Produktionsnummer (PPN)"@de ;
                   owl:versionInfo "PCP-on-Web 1 including property from merging Helmstedt data - 27.06.18"^^xsd:string .
	      
:praeses rdf:type owl:ObjectProperty ;
  rdfs:domain :Person ;
  rdfs:range :Disputation ;
  rdfs:derivedFrom <http://purl.org/pcp-on-web/ontology#praeses> ;
  rdfs:label "ist Praeses"@de, "is Praeses"@en ;
	rdfs:comment "Bezeichnet die Person, die während einer Disputation als Praeses auftritt und die Disputation leitet."@de, "Refers to the person who is the praeses - the head - of a disputation."@en .

:publisher rdf:type owl:ObjectProperty ;
  rdfs:subPropertyOf dc:creator;
  rdfs:range :Document ;
  rdfs:domain :Corporation, :Person ;
  rdfs:derivedFrom <http://purl.org/pcp-on-web/ontology#published> ;
  rdfs:label "ist Herausgeber"@de, "is publisher"@en ;
	rdfs:comment "Nennt Herausgeber eines Dokuments."@de, "Gives the publisher of a document."@en .	      
	      
:relatedDocument rdf:type owl:ObjectProperty ;
  rdfs:domain :StageOfLife;
  rdfs:range :Document;
  rdfs:label "Relevante Dokumente zu einem Lebensabschnitt"@de, "relevant documents of a stage of life"@en ;
	rdfs:comment "Ordnet einem Lebensabschnitt Dokumente zu, z.B. "@de, ".."@en .	      
	      
:reportHasChair rdf:type owl:ObjectProperty ;
  rdfs:domain :Report ;
  rdfs:range :Chair ;
  rdfs:label "Rechenschaftsbericht hat Lehrstuhl"@de, "report has chair"@en ;
	rdfs:comment "Ordnet einen Rechenschaftsbericht einem Lehrstuhl zu."@de, "Assigns a report to a chair."@en .
				     
:reportHasFaculty rdf:type owl:ObjectProperty ;
  rdfs:domain :Report ;
  rdfs:range :Faculty ;
  rdfs:label "Rechenschaftsbericht hat Fakultät"@de, "report has faculty"@en ;
	rdfs:comment "Ordnet einen Rechenschaftsbericht einer Fakultät zu."@de, "Assigns a report to a faculty."@en .

:respondent rdf:type owl:ObjectProperty ;
  rdfs:domain :Person ;
  rdfs:range :Disputation ;
  rdfs:derivedFrom <http://purl.org/pcp-on-web/ontology#respondent> ;
  rdfs:label "ist Respondent"@de, "is Respondent"@en ;
	rdfs:comment "Bezeichnet den Respondenten, der sich als Student der Disputation unterzieht."@de, "Refers to the respondent who as a student is undergoing the act of disputation."@en .   
	      
:stageOfLifeLocation rdf:type owl:ObjectProperty ;
  rdfs:domain :StageOfLife ;
  rdfs:range :Location ;
  rdfs:derivedFrom <http://purl.org/pcp-on-web/ontology#periodPlace> ;
  rdfs:label "Ort Lebensabschnitt"@de, "location of stage of life"@en ;
	rdfs:comment "Fügt einem Lebensabschnitt einer Person einen geografischen Ort zu."@de, "Adds a geographical location to a stage of life of a person."@en .
	      
:student rdf:type owl:ObjectProperty ;
  rdfs:domain :Professor ;
  rdfs:range :Student ;
  rdfs:label "ist Student"@de, "is student"@en ;
	rdfs:comment "Weist einen Professor als Student aus."@de, "Refers to the Professor as a student."@en .
	      
:spouse rdf:type owl:ObjectProperty ;
  rdfs:domain :Family ;
  rdfs:range :Professor ;
  rdfs:label "Ehepartner"@de, "spouse"@en ;
	rdfs:comment "Bezieht sich auf den Ehepartner (generisches Maskulinum) eines Professors."@de, "Refers to the spouse (generic masculine) of a professor."@en .

:tagged rdf:type owl:ObjectProperty ;
  rdfs:derivedFrom <http://purl.org/pcp-on-web/ontology#furtherInformation>, <http://purl.org/pcp-on-web/ontology#note>, <http://purl.org/pcp-on-web/ontology#keyword> ;
  rdfs:domain owl:Thing ;
  rdfs:range :Keyword ;
  rdfs:label "markiert"@de, "tagged"@en ;
	rdfs:comment "Gibt Informationen, die unspezifisch in Datenbanken unter Schlagworten, Kommentaren oder Notizen verborgen sind."@de, "Gives information that is unspecifically hidden in databases under keywords, comments or notes."@en .
	      
:territoryDocument rdf:type owl:ObjectProperty ;
  rdfs:domain :Territory ;
  rdfs:range :Document ;
  rdfs:label "hat Dokument"@de, "has Document"@en ;
	rdfs:comment "Bezieht sich auf das dazugehörige Dokument einer Ernennung, z.B. Bestallungsakte."@de, "Refers to documents of a vocation, like vocation files."@en .
	      
:vocates rdf:type owl:ObjectProperty ;
  rdfs:domain :Territory ;
  rdfs:range :Professor ;
  rdfs:label "beruft"@de, "vocates"@en ;
	rdfs:comment "Landesherrschaft beruft bzw. bestätigt und ernennt einen Professor."@de, "Territorial rulership vocates or confirms a Professor."@en .

:well-wisher rdf:type owl:ObjectProperty ;
  rdfs:domain :Dissertation ;
  rdfs:range :Person ;
  rdfs:derivedFrom <http://purl.org/pcp-on-web/ontology#wellWisher> ;
  rdfs:label "hat Gratulant"@de, "has well-wisher"@en ;
	rdfs:comment "Bezeichnet den Gratulanten einer Publikation, bspw. den Gratulanten eines Disputanten. Diese Gratulanten-Schriften befinden sich zumeist am Ende einer Dissertation."@de, "Refers to the well-wisher of a publication, e.g. the well-wisher to a disputant. These well-wishing writings are usually found at the end of a dissertation."@en .

	
#####################################################################################################################################################################

				
				     
:derivedFrom rdf:type owl:ObjectProperty ;
  rdfs:domain owl:Thing;
  rdfs:range owl:Thing ;
  rdfs:label "ist abgeleitet von"@de, "has been derived from"@en ;
	rdfs:comment "Wird für das Alignment genutzt."@de, "Wird für das Alignment genutzt."@en .
				     
	
